CoqOfRust/examples/default/examples/std_library_types/strings_raw_string_literals.v
@@ -15,6 +15,7 @@ fn main() {
     let longer_delimiter = r###"A string with "# in it. And even "##!"###;
     println!("{}", longer_delimiter);
 }
+"
 *)
 (* #[allow(dead_code)] - function was ignored by the compiler *)
 Definition main : M unit :=
